implement version 2

core/SerializableUpgradeNet.v
@@ -290,4 +290,230 @@ Module PBKV.
       end
       end.
   End VersionOne.
+
+
+  Module VersionTwo.
+    Inductive input := Put (k v : string) | Get (k : string) | Append (k s : string).
+    Definition input_serialize (i : input) : bytes :=
+      serialize 1 ++
+      match i with
+      | Put k v => serialize 0 ++ serialize k ++ serialize v
+      | Get k => serialize 1 ++ serialize k
+      | Append k s => serialize 2 ++ serialize k ++ serialize s
+      end.
+    Definition input_deserialize (bs : bytes) : option (input * bytes) :=
+      match deserialize bs with None => None
+      | Some (ver, rest) =>
+        if Nat.eq_dec ver 1
+        then
+          match deserialize rest with None => None
+          | Some (tag, rest) =>
+          match deserialize rest with None => None
+          | Some (k, rest) =>
+              match tag with
+              | 0 =>
+                match deserialize rest with None => None
+                | Some (v,rest) => Some (Put k v, rest)
+                end
+              | 1 => Some (Get k, rest)
+              | 2 =>
+                match deserialize rest with None => None
+                | Some (s,rest) => Some (Append k s, rest)
+                end
+              | _ => None
+              end
+          end
+          end
+        else None
+      end.
+    Instance input_Serializer : Serializer input :=
+      {| serialize := input_serialize;
+         deserialize := input_deserialize
+      |}.
+    unfold input_serialize, input_deserialize.
+    intros.
+    destruct x;
+       rewrite !app_assoc_reverse;
+       now rewrite !Serialize_reversible.
+    Defined.
+
+    Inductive msg := Cmd (i : input) | Ack.
+    Definition msg_serialize (m : msg) : bytes :=
+      serialize 0 ++
+      match m with
+      | Cmd i => serialize true ++ serialize i
+      | Ack => serialize false
+      end.
+    Definition msg_deserialize (bs : bytes) : option (msg * bytes) :=
+        match deserialize bs with None => None
+        | Some (ver, rest)  =>
+        match deserialize rest with None => None
+        | Some (b, rest) =>
+          if Nat.eq_dec ver 0
+          then if b:bool
+               then match deserialize rest with None => None
+                                           | Some (i, rest) => Some (Cmd i, rest)
+                    end
+               else Some (Ack, rest)
+          else None
+        end
+        end.
+    Instance msg_Serializer : Serializer msg :=
+      {| serialize := msg_serialize;
+         deserialize := msg_deserialize
+      |}.
+    unfold msg_serialize, msg_deserialize.
+    intros.
+    destruct x;
+      rewrite !app_assoc_reverse;
+      now rewrite !Serialize_reversible.
+    Defined.
+
+    Inductive output := ResGet (k v : string)
+                      | ResPut (k old_v v : string)
+                      | ResAppend (k s old_v v : string).
+    Definition output_serialize (o : output) : bytes :=
+      serialize 1 ++
+      match o with
+      | ResGet k v => serialize 0 ++ serialize k ++ serialize v
+      | ResPut k old_v v => serialize 1 ++ serialize k ++ serialize old_v ++ serialize v
+      | ResAppend k s old_v v => serialize 2 ++ serialize k ++ serialize s ++
+                                serialize old_v ++ serialize v
+      end.
+    Definition output_deserialize (bs : bytes) : option (output * bytes) :=
+      match deserialize bs with None => None
+      | Some (ver, rest) =>
+        if Nat.eq_dec ver 1
+        then
+          match deserialize rest with None => None
+          | Some (tag, rest) =>
+            match deserialize rest with None => None
+            | Some (k, rest) =>
+            match tag with
+            | 0 =>
+              match deserialize rest with None => None
+              | Some (v, rest) => Some (ResGet k v, rest)
+              end
+            | 1 =>
+              match deserialize rest with None => None
+              | Some (old_v, rest) =>
+              match deserialize rest with None => None
+              | Some (v, rest) => Some (ResPut k old_v v, rest)
+              end
+              end
+            | 2 =>
+              match deserialize rest with None => None
+              | Some (s, rest) =>
+              match deserialize rest with None => None
+              | Some (old_v, rest) =>
+              match deserialize rest with None => None
+              | Some (v, rest) => Some (ResAppend k s old_v v, rest)
+              end
+              end
+              end
+            | _ => None
+            end
+            end
+          end
+        else None
+      end.
+    Instance output_Serializer : Serializer output :=
+      {| serialize := output_serialize;
+         deserialize := output_deserialize
+      |}.
+    unfold output_serialize, output_deserialize.
+    intros.
+    destruct x;
+      rewrite !app_assoc_reverse;
+      now rewrite !Serialize_reversible.
+    Qed.
+
+    Record data := Data { db : list (string * string);
+                          log : list input;
+                          nextIndex : nat
+                        }.
+    Definition data_serialize (d : data) : bytes :=
+      serialize (db d) ++ serialize (log d) ++ serialize (nextIndex d).
+    Definition data_deserialize (bs : bytes) : option (data * bytes) :=
+      match deserialize bs with None => None
+      | Some (db, rest) =>
+      match deserialize rest with None => None
+      | Some (log, rest) =>
+      match deserialize rest with None => None
+      | Some (ni, rest) => Some (Data db log ni, rest)
+      end
+      end
+      end.
+    Instance data_Serializer : Serializer data :=
+      {| serialize := data_serialize;
+         deserialize := data_deserialize
+      |}.
+    unfold data_serialize, data_deserialize.
+    intros.
+    destruct x.
+    rewrite !app_assoc_reverse.
+    now rewrite !Serialize_reversible.
+    Qed.
+
+    Definition nop (s : bytes) : bytes * list (name * bytes) * list bytes := (s, [], []).
+
+    Definition handleInput (n : name) (i : bytes) (s : bytes) :
+        bytes * list (name * bytes) * list bytes :=
+      match deserialize s with None => nop s
+      | Some (s, _) =>
+      match deserialize i with None => nop (serialize s)
+      | Some (i, _) =>
+      match n with
+      | Primary =>
+        let log' := log s ++ [i] in
+        let ms := if Nat.eq_dec (length (log s)) (nextIndex s)
+                  then [(Backup, serialize (Cmd i))]
+                  else [] in
+        (serialize (Data (db s) log' (nextIndex s)), ms, [])
+      | Backup => nop (serialize s)
+      end
+      end
+      end.
+
+    Definition execute (i : input) (db : list (string * string))
+        : output * list (string * string) :=
+      match i with
+      | Put k v => let old_v := assoc_default String.string_dec db String.EmptyString k in
+                  let db' := assoc_set String.string_dec db k v in
+                  (ResPut k old_v v, db')
+      | Get k => let v := assoc_default String.string_dec db String.EmptyString k in
+                (ResGet k v, db)
+      | Append k s => let old_v := assoc_default String.string_dec db String.EmptyString k in
+                     let v := String.append old_v s in
+                     let db' := assoc_set String.string_dec db k v in
+                     (ResAppend k s old_v v, db')
+      end.
+
+    Definition handleMsg (n : name) (m : bytes) (s : bytes) :
+        bytes * list (name * bytes) * list bytes :=
+      match deserialize s with None => nop s
+      | Some (s, _) =>
+      match deserialize m with None => nop (serialize s)
+      | Some (m, _) =>
+      match n, m with
+      | Primary, Ack =>
+        match nth_error (log s) (nextIndex s) with None => nop (serialize s)
+        | Some i => let (o, db') := execute i (db s) in
+                   let ni' := S (nextIndex s) in
+                   let ms := match nth_error (log s) ni' with
+                             | None => []
+                             | Some i' => [(Backup, serialize (Cmd i))]
+                             end
+                   in (serialize (Data db' (log s) ni'), ms, [serialize o])
+        end
+      | Backup, Cmd i => let log' := log s ++ [i] in
+                        let (_, db') := execute i (db s) in
+                        (serialize (Data db' log' (nextIndex s)),
+                         [(Primary, serialize Ack)],
+                         [])
+      | _, _ => nop (serialize s)
+      end
+      end
+      end.
+  End VersionTwo.
 End PBKV.
